Extend ArrayQuery interface to expose [goodSize] in negative case; include skeleton of a loop in Server

examples/comparison/Server.v
@@ -31,6 +31,11 @@ Fixpoint encodeAll (rs : list req) : list W :=
 
 (* Helper functions to express semantics of requests *)
 
+Definition valueIsGe (data : list W) (index lower : W) : W :=
+  if le_lt_dec (length data) (wordToNat index)
+    then $0
+    else if wlt_dec (Array.sel data index) lower then $0 else $1.
+
 Definition wmax (w w' : W) : W :=
   if wlt_dec w' w then w' else w.
 
@@ -40,10 +45,10 @@ Fixpoint maxInRange (lower upper : W) (data : list W) : W :=
     | w :: ws =>
       let max := maxInRange lower upper ws in
         if wlt_dec w lower
-          then if wlt_dec upper w
-            then wmax w max
-            else max
-          else max
+          then max
+          else if wlt_dec upper w
+            then max
+            else wmax w max
   end.
 
 Fixpoint collectBelow (upper : W) (data acc : list W) : list W :=
@@ -51,20 +56,15 @@ Fixpoint collectBelow (upper : W) (data acc : list W) : list W :=
     | nil => acc
     | w :: ws =>
       if wlt_dec upper w
-        then collectBelow upper ws (w :: acc)
-        else collectBelow upper ws acc
+        then collectBelow upper ws acc
+        else collectBelow upper ws (w :: acc)
   end.
 
 (* Mathematical function to compute the proper response to a request,
  * in terms of a transformation on a list of output values. *)
 Definition response (data : list W) (acc : list W) (r : req) : list W :=
   match r with
-    | ValueIsGe index lower =>
-      if le_lt_dec (length data) (wordToNat index)
-        then acc
-        else if wlt_dec (Array.sel data index) lower
-          then $1 :: acc
-          else $0 :: acc
+    | ValueIsGe index lower => valueIsGe data index lower :: acc
     | MaxInRange lower upper =>
       maxInRange lower upper data :: acc
     | CollectBelow lower upper =>
@@ -85,7 +85,8 @@ Definition mainS := SPEC("cmd", "cmdLen", "data", "dataLen") reserving 13
 Definition m := bimport [[ "malloc"!"malloc" @ [mallocS] ]]
   bmodule "m" {{
     bfunction "main"("cmd", "cmdLen", "data", "dataLen",
-                    "output", "position", "posn", "lower", "upper") [mainS]
+                     "output", "position", "posn", "lower", "upper",
+                     "index", "value", "res") [mainS]
       "output" <- 0;;
       "position" <- 0;;
 
@@ -98,12 +99,34 @@ Definition m := bimport [[ "malloc"!"malloc" @ [mallocS] ]]
          * sll (responseAll d r out) R]
       While ("position" < "cmdLen") {
         Match "cmd" Size "cmdLen" Position "position" {
+          (* ValueIsGe *)
           Case (0 ++ "posn" ++ "lower")
+            "res" <- 0;;
+
+            [Al rdone, Al r, Al out,
+              After prefix Approaching all
+                PRE[V] array (rdone ++ encodeAll (ValueIsGe (V "posn") (V "lower") :: r)) (V "cmd")
+                  * mallocHeap * sll out (V "output") * [| V "position" = natToW (length rdone + 3) |]
+                  * [| V "cmdLen" = (length rdone + 3 + length (encodeAll r))%nat |]
+                  * [| V "dataLen" = length all |]
+                  * [| V "res" = valueIsGe prefix (V "posn") (V "lower") |]
+                  * [| goodSize (length rdone + 3 + length (encodeAll r) + 3) |]
+                POST[R] array (rdone ++ encodeAll (ValueIsGe (V "posn") (V "lower") :: r)) (V "cmd")
+                  * mallocHeap * sll (responseAll all (ValueIsGe (V "posn") (V "lower") :: r) out) R ]
+            For "index" Holding "value" in "data" Size "dataLen"
+              Where ((Index = "posn") && (Value >= "lower")) {
+              Diverge
+            };;
+
             Diverge
           end;;
+
+          (* MaxInRange *)
           Case (1 ++ "lower" ++ "upper")
             Diverge
           end;;
+
+          (* CollectBelow *)
           Case (2 ++ "lower" ++ "upper")
             Diverge
           end
@@ -137,18 +160,155 @@ Hint Extern 1 (length _ = 0) =>
 
 Hint Rewrite responseAll_nil using solve [ auto ] : Server.
 
+Hint Rewrite natToW_plus : Server.
+
+Lemma triple' : forall (x : W) y,
+  x ^+ natToW (S (S (S y))) = x ^+ $3 ^+ natToW y.
+  intros; do 3 match goal with
+                 | [ |- context[S ?X] ] => rewrite (natToW_S X)
+               end; words.
+Qed.
+
+Lemma triple : forall (x : W) (ws : list W),
+  x ^+ natToW (S (S (S (length ws)))) = x ^+ $3 ^+ natToW (length ws).
+  intros; rewrite triple'; auto.
+Qed.
+
+Hint Rewrite triple : Server.
+
+Ltac eta_evar T k :=
+  match eval cbv beta in T with
+    | unit => k tt
+    | @sigT ?A ?F =>
+      let x' := fresh in evar (x' : A); let x := eval unfold x' in x' in clear x';
+        eta_evar (F x) ltac:(fun v => k (existT F x v))
+    | _ =>
+      idtac "BYE";
+        let x' := fresh in evar (x' : T); let x := eval unfold x' in x' in clear x';
+          k x
+  end.
+
+Ltac parse1 solver :=
+  match goal with
+    | [ H : forall (a : _ -> _), _ |- _ ] =>
+      especialize H; post;
+      match goal with
+        | [ H : interp ?specs (?P ---> ?Q)%PropX |- _ ] =>
+          let H' := fresh in assert (H' : interp specs P) by (propxFo; step auto_ext || solver);
+            specialize (Imply_sound H H'); clear H H'; intro H
+      end; propxFo; autorewrite with StreamParse in *; simpl in *
+
+    | [ H : interp _ (![ _ ] _) |- _ ] => eapply Wrap.sepFormula_Mem in H; [ | eassumption ]
+  end.
+
+Lemma suffix_app' : forall (ls2 ls1 : list W),
+  suffix (length ls1) (ls1 ++ ls2) = ls2.
+  induction ls1; simpl; intuition.
+Qed.
+
+Lemma suffix_app : forall (ls1 ls2 : list W) (v : W),
+  v = natToW (length ls1)
+  -> goodSize (length ls1)
+  -> suffix (wordToNat v) (ls1 ++ ls2) = ls2.
+  intros; subst; rewrite wordToNat_natToW_goodSize; auto; apply suffix_app'.
+Qed.
+
+Ltac use_match := try rewrite suffix_app in * by (assumption || eapply goodSize_weaken; eauto);
+  try match goal with
+        | [ H : match encodeAll ?E with nil => False | _ => _ end |- _ ] =>
+          destruct E as [ | [ ] ]; simpl in *; intuition (try discriminate); subst
+      end; reveal_slots; evaluate hints.
+
+Ltac multi_ex :=
+  try match goal with
+        | [ _ : sigT _ |- _ ] =>
+          repeat match goal with
+                   | [ x : sigT _ |- _ ] => destruct x
+                 end; simpl in *
+      end;
+  try match goal with
+        | [ |- @Logic.ex ?T _ ] =>
+          match T with
+            | sigT _ => eta_evar T ltac:(fun v => exists v; simpl)
+          end
+      end.
+
+Hint Rewrite app_length : Server.
+
 Ltac finish :=
   repeat match goal with
            | [ H : sel _ _ = _ |- _ ] => rewrite H in *
            | [ H : Regs _ _ = sel _ _ |- _ ] => rewrite H in *
          end; try rewrite wordToNat_natToW_goodSize by (eapply goodSize_weaken; eauto);
-  eauto; try rewrite app_length; eauto; simpl;
-    autorewrite with Server;
-      try solve [ eapply goodSize_weaken; eauto | step hints ].
+  eauto; autorewrite with Server; simpl; autorewrite with Server; eauto; simpl;
+    try solve [ auto | eapply goodSize_weaken; eauto | step hints ].
+
+
+Lemma switch_sides : forall w n,
+  wordToNat w = n
+  -> natToW n = w.
+  intros; subst; apply natToWord_wordToNat.
+Qed.
+
+Hint Immediate switch_sides.
+
+Hint Extern 1 (weqb _ _ = true) => apply weqb_true_iff.
+Hint Resolve wleb_true.
+
+Lemma selN_beginning : forall (w : W) (ws' : list W) (ws : list W) i,
+  (i < length ws)%nat
+  -> Array.selN (ws ++ w :: ws') i = Array.selN ws i.
+  induction ws; destruct i; simpl; intuition.
+Qed.
+
+Lemma sel_beginning : forall (ws : list W) (w : W) (ws' : list W) i,
+  goodSize (length ws)
+  -> i < natToW (length ws)
+  -> Array.sel (ws ++ w :: ws') i = Array.sel ws i.
+  unfold Array.sel; intros; apply selN_beginning; nomega.
+Qed.
+
+Lemma valueIsGe_skip : forall v ws this posn lower,
+  v = valueIsGe ws posn lower
+  -> goodSize (length ws)
+  -> (weqb (length ws) posn = true -> wleb lower this = true -> False)
+  -> v = valueIsGe (ws ++ this :: nil) posn lower.
+  unfold valueIsGe; intros; autorewrite with Server; simpl.
+  destruct (le_lt_dec (length ws) (wordToNat posn));
+    destruct (le_lt_dec (length ws + 1) (wordToNat posn)); auto; try omega; [
+      assert (wordToNat posn = length ws) by omega;
+        replace posn with (natToW (length ws)) by auto;
+          rewrite sel_middle by auto;
+            destruct (wlt_dec this lower); eauto; elimtype False; eauto
+      | destruct (eq_nat_dec (wordToNat posn) (length ws)); [
+        replace posn with (natToW (length ws)) by auto;
+          rewrite sel_middle by auto; nomega
+        | rewrite sel_beginning; auto; nomega ] ].
+Qed.
+
+Hint Immediate valueIsGe_skip.
 
 
 Theorem ok : moduleOk m.
 Proof.
-  vcgen; abstract (parse0; for0;
-    post; evaluate hints; repeat (parse1; evaluate hints); sep hints; finish).
+  vcgen; parse0; for0.
+
+  Ltac t := post; evaluate hints; repeat (parse1 finish; use_match); multi_ex; sep hints; finish.
+
+  t.
+  t.
+  t.
+  t.
+  t.
+  t.
+  t.
+  t.
+  t.
+  t.
+  t.
+  t.
+  t.
+  t.
+  t.
+  t.
 Qed.
